concurrency/fineConc_safe.v
@@ -547,7 +547,7 @@ Module FineConcSafe.
 
   End Safety.
 End FineConcSafe.
-
+End FineConcSafe.
 
 
 
